src/examples/mutex/wait_set.v
@@ -15,6 +15,12 @@ Ltac lookup_simp :=
     end;
   try congruence.
 
+(*|
+===========
+Wake set
+===========
+|*)
+
 Definition wait_pc pc :=
   pc = pc.lock_cas ∨
   pc = pc.futex_wait ∨
@@ -173,3 +179,66 @@ Proof. set_solver. Qed.
 
 #[export]
 Hint Resolve wait_set_remove_subset wait_set_remove_eq : core.
+Hint Rewrite wait_set_remove_eq using (by eauto) : pc.
+
+(*|
+===========
+Wake set
+===========
+|*)
+
+Definition wake_set (tp: gmap Tid pc.t) : gset Tid :=
+  dom (filter (λ '(_, pc), pc = pc.unlock_wake) tp).
+
+Lemma elem_wake_set tp t :
+  t ∈ wake_set tp ↔ tp !! t = Some pc.unlock_wake.
+Proof.
+  rewrite /wake_set.
+  rewrite elem_of_dom filter_is_Some. naive_solver.
+Qed.
+
+Lemma elem_wake_set_2 tp t :
+  tp !! t = Some pc.unlock_wake →
+  t ∈ wake_set tp.
+Proof.
+  apply elem_wake_set.
+Qed.
+
+Lemma not_elem_wake_set tp t pc :
+  tp !! t = Some pc →
+  pc ≠ pc.unlock_wake →
+  t ∉ wake_set tp.
+Proof.
+  rewrite elem_wake_set.
+  naive_solver.
+Qed.
+
+#[export]
+Hint Resolve elem_wake_set_2 not_elem_wake_set : core.
+
+Lemma wake_set_remove tp t pc' :
+  pc' ≠ pc.unlock_wake →
+  wake_set (<[t := pc']> tp) = wake_set tp ∖ {[t]}.
+Proof.
+  intros.
+  apply gset_ext => t'.
+  rewrite /wake_set. rewrite elem_of_difference !elem_of_dom !filter_is_Some.
+  rewrite elem_of_singleton.
+  destruct (decide (t = t')); lookup_simp; naive_solver.
+Qed.
+
+#[export]
+Hint Rewrite wake_set_remove using (by auto) : pc.
+
+Lemma wake_set_add tp t :
+  wake_set (<[t := pc.unlock_wake]> tp) = wake_set tp ∪ {[t]}.
+Proof.
+  intros.
+  apply gset_ext => t'.
+  rewrite /wake_set. rewrite elem_of_union !elem_of_dom !filter_is_Some.
+  rewrite elem_of_singleton.
+  destruct (decide (t = t')); lookup_simp; naive_solver.
+Qed.
+
+#[export]
+Hint Rewrite wake_set_add : pc.
